Phi_Examples/Binary_Trees.thy
@@ -297,21 +297,21 @@ proc lookup_bintree:
   obtain L node R where tree_def[simp]: \<open>tree = \<langle>L, node, R\<rangle>\<close> by auto_sledgehammer \<semicolon>
   \<t>\<r>\<a>\<n>\<s>\<f>\<o>\<r>\<m>\<s>_\<t>\<o> \<open>\<o>\<p>\<e>\<n>(1)\<close> \<exists>a\<^sub>L, a\<^sub>R \<semicolon>
  
-  val k' \<leftarrow> $addr.data.k ! \<semicolon>
-  if (eq ($k', $k)) \<medium_left_bracket>
-    val ret \<leftarrow> $addr.data.v ! \<semicolon>
+  val k' \<leftarrow> addr.data.k \<semicolon>
+  if (eq (k', k)) \<medium_left_bracket>
+    val ret \<leftarrow> addr.data.v \<semicolon>
     \<m>\<a>\<k>\<e>\<s>(1) \<open>BinTree addr _ _\<close> \<semicolon>
-    return ($ret)
+    return (ret)
   \<medium_right_bracket>
   \<medium_left_bracket>
-    if (cmp ($k, $k')) \<medium_left_bracket>
-      lookup_bintree ($addr.left !, $k) \<rightarrow> val ret \<semicolon>
+    if (cmp (k, k')) \<medium_left_bracket>
+      lookup_bintree (addr.left, k) \<rightarrow> val ret \<semicolon>
       \<m>\<a>\<k>\<e>\<s>(1) \<open>BinTree addr _ _\<close> \<semicolon>
-      return ($ret)
+      return (ret)
     \<medium_right_bracket> \<medium_left_bracket>
-      lookup_bintree ($addr.right !, $k) \<rightarrow> val ret \<semicolon>
+      lookup_bintree (addr.right, k) \<rightarrow> val ret \<semicolon>
       \<open>BinTree a\<^sub>L _ _\<close> \<m>\<a>\<k>\<e>\<s>(1) \<open>BinTree addr _ _\<close> \<semicolon>
-      return ($ret)
+      return (ret)
     \<medium_right_bracket> \<semicolon>
   \<medium_right_bracket>
 \<medium_right_bracket> .
@@ -322,7 +322,7 @@ proc (nodef) lookup_bst:
   output   \<open>the (f k) \<Ztypecolon> \<v>\<a>\<l> V\<heavy_comma> f \<Ztypecolon> Bin_Search_Tree addr TY\<^sub>K TY\<^sub>V K V\<close>
   unfolding Bin_Search_Tree.unfold
 \<medium_left_bracket>
-  lookup_bintree ($addr, $k)
+  lookup_bintree (addr, k)
 \<medium_right_bracket> .
 
 
@@ -341,20 +341,20 @@ proc defined_bintree:
     obtain L node R where tree_def[simp]: \<open>tree = \<langle>L, node, R\<rangle>\<close> by auto_sledgehammer \<semicolon>
     \<t>\<r>\<a>\<n>\<s>\<f>\<o>\<r>\<m>\<s>_\<t>\<o> \<open>\<o>\<p>\<e>\<n>(1)\<close> \<exists>a\<^sub>L, a\<^sub>R \<semicolon>
 
-    val k' \<leftarrow> $addr.data.k ! \<semicolon>
-    if (eq ($k', $k)) \<medium_left_bracket>
+    val k' \<leftarrow> addr.data.k \<semicolon>
+    if (eq (k', k)) \<medium_left_bracket>
       \<m>\<a>\<k>\<e>\<s>(1) \<open>BinTree addr _ _\<close> \<semicolon>
       return (True)
     \<medium_right_bracket>
     \<medium_left_bracket>
-      if (cmp ($k, $k')) \<medium_left_bracket>
-        val ret \<leftarrow> defined_bintree ($addr.left !, $k) \<semicolon>
+      if (cmp (k, k')) \<medium_left_bracket>
+        val ret \<leftarrow> defined_bintree (addr.left, k) \<semicolon>
         \<open>BinTree a\<^sub>L _ _\<close> \<m>\<a>\<k>\<e>\<s>(1) \<open>BinTree addr _ _\<close> \<semicolon>
-        return ($ret)
+        return (ret)
       \<medium_right_bracket> \<medium_left_bracket> 
-        val ret \<leftarrow> defined_bintree ($addr.right !, $k) \<semicolon>
+        val ret \<leftarrow> defined_bintree (addr.right, k) \<semicolon>
         \<open>BinTree a\<^sub>L _ _\<close> \<m>\<a>\<k>\<e>\<s>(1) \<open>BinTree addr _ _\<close> \<semicolon>
-        return ($ret)
+        return (ret)
       \<medium_right_bracket> \<semicolon>
     \<medium_right_bracket>
   \<medium_right_bracket>
@@ -366,7 +366,7 @@ proc (nodef) defined_bst:
   output \<open>k \<in> dom f \<Ztypecolon> \<v>\<a>\<l> \<bool>\<heavy_comma> f \<Ztypecolon> Bin_Search_Tree addr TY\<^sub>K TY\<^sub>V K V\<close>
   unfolding Bin_Search_Tree.unfold
 \<medium_left_bracket>
-  defined_bintree ($addr, $k)
+  defined_bintree (addr, k)
 \<medium_right_bracket> .
 
 
@@ -389,30 +389,30 @@ proc insert_bintree:
 \<medium_left_bracket>
   if \<open>$addr = 0\<close> \<medium_left_bracket>
       val ret \<leftarrow> calloc1 \<open>Bst_Node\<close> \<semicolon>
-      $ret.data.k := $k \<semicolon>
-      $ret.data.v := $v \<semicolon>
+      ret.data.k := k \<semicolon>
+      ret.data.v := v \<semicolon>
       \<m>\<a>\<k>\<e>\<s>(1) \<open>\<langle>\<langle>\<rangle>, (k,v), \<langle>\<rangle>\<rangle> \<Ztypecolon> BinTree addrb (\<k>\<v>_\<p>\<a>\<i>\<r> TY\<^sub>K TY\<^sub>V) \<lbrace> k: K, v: V \<rbrace>\<close> \<semicolon>
-      return ($ret)
+      return (ret)
   \<medium_right_bracket> \<medium_left_bracket>
       obtain L node R where tree_def[simp]: \<open>tree = \<langle>L, node, R\<rangle>\<close> by auto_sledgehammer \<semicolon>
       \<t>\<r>\<a>\<n>\<s>\<f>\<o>\<r>\<m>\<s>_\<t>\<o> \<open>\<o>\<p>\<e>\<n>(1)\<close> \<exists>a\<^sub>L, a\<^sub>R \<semicolon>
 
-      val k' \<leftarrow> $addr.data.k ! \<semicolon>
-      if (eq ($k', $k)) \<medium_left_bracket>
-          $addr.data.v := $v \<semicolon>
+      val k' \<leftarrow> addr.data.k \<semicolon>
+      if (eq (k', k)) \<medium_left_bracket>
+          addr.data.v := v \<semicolon>
           \<m>\<a>\<k>\<e>\<s>(1) \<open>BinTree addr _ _\<close>  \<semicolon>
-          return ($addr)
+          return (addr)
       \<medium_right_bracket> \<medium_left_bracket>
-          if (cmp ($k, $k')) \<medium_left_bracket>
-              insert_bintree ($addr.left !, $k, $v) \<rightarrow> val a\<^sub>L' \<semicolon>
-              $addr.left := $a\<^sub>L' \<semicolon>
+          if (cmp (k, k')) \<medium_left_bracket>
+              insert_bintree (addr.left, k, v) \<rightarrow> val a\<^sub>L' \<semicolon>
+              addr.left := a\<^sub>L' \<semicolon>
               \<m>\<a>\<k>\<e>\<s>(1) \<open>BinTree addr _ _\<close> \<semicolon>
-              return ($addr)
+              return (addr)
           \<medium_right_bracket> \<medium_left_bracket>
-              insert_bintree ($addr.right !, $k, $v) \<rightarrow> val a\<^sub>R' \<semicolon>
-              $addr.right := $a\<^sub>R' \<semicolon>
+              insert_bintree (addr.right, k, v) \<rightarrow> val a\<^sub>R' \<semicolon>
+              addr.right := a\<^sub>R' \<semicolon>
               \<open>BinTree a\<^sub>L _ _\<close> \<m>\<a>\<k>\<e>\<s>(1) \<open>BinTree addr _ _\<close> \<semicolon>
-              return ($addr)
+              return (addr)
           \<medium_right_bracket>
       \<medium_right_bracket>
   \<medium_right_bracket>
@@ -429,7 +429,7 @@ proc (nodef) insert_bst:
           \<s>\<u>\<b>\<j> addr'. \<top>\<close>
   unfolding Bin_Search_Tree.unfold
 \<medium_left_bracket>
-  insert_bintree ($addr, $k, $v)
+  insert_bintree (addr, k, v)
 \<medium_right_bracket> .
 
 
@@ -437,7 +437,7 @@ proc Max:
   input  \<open>x \<Ztypecolon> \<v>\<a>\<l> \<nat>\<heavy_comma> y \<Ztypecolon> \<v>\<a>\<l> \<nat>\<close>
   output \<open>max x y \<Ztypecolon> \<v>\<a>\<l> \<nat>\<close>
 \<medium_left_bracket>
-  if ($x < $y) \<medium_left_bracket> $y \<medium_right_bracket> \<medium_left_bracket> $x \<medium_right_bracket>
+  if (x < y) \<medium_left_bracket> y \<medium_right_bracket> \<medium_left_bracket> x \<medium_right_bracket>
 \<medium_right_bracket> .
 
 
@@ -454,9 +454,9 @@ proc height_of:
   \<medium_right_bracket> \<medium_left_bracket>
       obtain L node R where tree_def[simp]: \<open>tree = \<langle>L, node, R\<rangle>\<close> by auto_sledgehammer \<semicolon>
       \<t>\<r>\<a>\<n>\<s>\<f>\<o>\<r>\<m>\<s>_\<t>\<o> \<open>\<o>\<p>\<e>\<n>(1)\<close> \<semicolon>
-      $addr.data.v.height ! \<rightarrow> val ret \<semicolon>
+      addr.data.v.height \<rightarrow> val ret \<semicolon>
       \<m>\<a>\<k>\<e>\<s>(1) \<open>tree \<Ztypecolon> BinTree addr _ _\<close> \<semicolon>
-      return ($ret)
+      return (ret)
   \<medium_right_bracket>
 \<medium_right_bracket> .
 
@@ -481,48 +481,48 @@ proc maintain_i:
 
   \<t>\<r>\<a>\<n>\<s>\<f>\<o>\<r>\<m>\<s>_\<t>\<o> \<open>OPEN 1 _\<close> \<exists>a\<^sub>B, a\<^sub>E \<semicolon>                                                 (*for reasoning, \<Omega>*)
 
-  val B \<leftarrow> $a\<^sub>D.left ! \<semicolon>
-  val E \<leftarrow> $a\<^sub>D.right ! \<semicolon>
-  val H\<^sub>B \<leftarrow> height_of ($B) \<semicolon>
-  val H\<^sub>E \<leftarrow> height_of ($E) \<semicolon>
+  val B \<leftarrow> a\<^sub>D.left \<semicolon>
+  val E \<leftarrow> a\<^sub>D.right \<semicolon>
+  val H\<^sub>B \<leftarrow> height_of (B) \<semicolon>
+  val H\<^sub>E \<leftarrow> height_of (E) \<semicolon>
 
-  if ($H\<^sub>B = $H\<^sub>E + 2) \<medium_left_bracket>
+  if (H\<^sub>B = H\<^sub>E + 2) \<medium_left_bracket>
       obtain A k\<^sub>B h\<^sub>B v\<^sub>B C where B[simp]: \<open>B = \<langle>A, (k\<^sub>B, h\<^sub>B, v\<^sub>B), C\<rangle>\<close> by auto_sledgehammer \<semicolon> (*this line and the*)
       \<open>BinTree a\<^sub>B _ _\<close> \<t>\<r>\<a>\<n>\<s>\<f>\<o>\<r>\<m>\<s>_\<t>\<o> \<open>\<o>\<p>\<e>\<n>(1)\<close> \<exists>a\<^sub>A, a\<^sub>C \<semicolon>                                        (*next line, for reasoning, one \<Omega>*)
 
-      val A \<leftarrow> $B.left ! \<semicolon>
-      val C \<leftarrow> $B.right ! \<semicolon>
-      val H\<^sub>A \<leftarrow> height_of ($A) \<semicolon>
-      val H\<^sub>C \<leftarrow> height_of ($C) \<semicolon>
+      val A \<leftarrow> B.left \<semicolon>
+      val C \<leftarrow> B.right \<semicolon>
+      val H\<^sub>A \<leftarrow> height_of (A) \<semicolon>
+      val H\<^sub>C \<leftarrow> height_of (C) \<semicolon>
 
-      if ($H\<^sub>C \<le> $H\<^sub>A) \<medium_left_bracket>
+      if (H\<^sub>C \<le> H\<^sub>A) \<medium_left_bracket>
 
-          $a\<^sub>D.left := $C \<semicolon>
-          val H\<^sub>D' \<leftarrow> Max($H\<^sub>C, $H\<^sub>E) + 1 \<semicolon>
-          $a\<^sub>D.data.v.height := $H\<^sub>D' \<semicolon>
-          $B.right := $a\<^sub>D \<semicolon>
-          $B.data.v.height := Max($H\<^sub>A, $H\<^sub>D') + 1 \<semicolon>
+          a\<^sub>D.left := C \<semicolon>
+          val H\<^sub>D' \<leftarrow> Max(H\<^sub>C, H\<^sub>E) + 1 \<semicolon>
+          a\<^sub>D.data.v.height := H\<^sub>D' \<semicolon>
+          B.right := a\<^sub>D \<semicolon>
+          B.data.v.height := Max(H\<^sub>A, H\<^sub>D') + 1 \<semicolon>
 
           \<open>BinTree a\<^sub>E _ _\<close> \<open>BinTree a\<^sub>C _ _\<close> \<m>\<a>\<k>\<e>\<s>(1) \<open>BinTree a\<^sub>D _ _\<close> \<semicolon>                 (*for reasoning, \<Omega>*)
           \<open>BinTree a\<^sub>A _ _\<close> \<m>\<a>\<k>\<e>\<s>(1) \<open>BinTree a\<^sub>B _ _\<close> \<semicolon>                                                  (*for reasoning, \<Omega>*)
  
-          return ($B) certified by (auto simp add: fun_eq_iff map_add_def split: option.split; auto_sledgehammer) (*Tac-1n-2m*)
+          return (B) certified by (auto simp add: fun_eq_iff map_add_def split: option.split; auto_sledgehammer) (*Tac-1n-2m*)
       \<medium_right_bracket>
       \<medium_left_bracket>
           obtain C\<^sub>L k\<^sub>C h\<^sub>C v\<^sub>C C\<^sub>R where C[simp]: \<open>C = \<langle>C\<^sub>L, (k\<^sub>C, h\<^sub>C, v\<^sub>C), C\<^sub>R\<rangle>\<close> by auto_sledgehammer \<semicolon>  (*this line and the next*)
           \<open>BinTree a\<^sub>C _ _\<close> \<t>\<r>\<a>\<n>\<s>\<f>\<o>\<r>\<m>\<s>_\<t>\<o> \<open>\<o>\<p>\<e>\<n>(1)\<close> \<exists>a\<^sub>C\<^sub>L, a\<^sub>C\<^sub>R \<semicolon>                                           (*line, for reasoning, one \<Omega>*)
 
-          val C\<^sub>L \<leftarrow> $C.left ! \<semicolon>
-          val C\<^sub>R \<leftarrow> $C.right ! \<semicolon>
-          $B.right := $C\<^sub>L \<semicolon>
-          val H\<^sub>B' \<leftarrow> Max($H\<^sub>A, height_of($C\<^sub>L)) + 1 \<semicolon>
-          $B.data.v.height := $H\<^sub>B'\<semicolon>
-          $a\<^sub>D.left := $C.right ! \<semicolon>
-          val H\<^sub>D' \<leftarrow> Max($H\<^sub>E, height_of($C\<^sub>R)) + 1 \<semicolon>
-          $a\<^sub>D.data.v.height := $H\<^sub>D' \<semicolon>
-          $C.left := $B \<semicolon>
-          $C.right := $a\<^sub>D \<semicolon>
-          $C.data.v.height := Max($H\<^sub>B', $H\<^sub>D') + 1 \<semicolon>
+          val C\<^sub>L \<leftarrow> C.left \<semicolon>
+          val C\<^sub>R \<leftarrow> C.right \<semicolon>
+          B.right := C\<^sub>L \<semicolon>
+          val H\<^sub>B' \<leftarrow> Max(H\<^sub>A, height_of(C\<^sub>L)) + 1 \<semicolon>
+          B.data.v.height := H\<^sub>B'\<semicolon>
+          a\<^sub>D.left := C.right \<semicolon>
+          val H\<^sub>D' \<leftarrow> Max(H\<^sub>E, height_of(C\<^sub>R)) + 1 \<semicolon>
+          a\<^sub>D.data.v.height := H\<^sub>D' \<semicolon>
+          C.left := B \<semicolon>
+          C.right := a\<^sub>D \<semicolon>
+          C.data.v.height := Max(H\<^sub>B', H\<^sub>D') + 1 \<semicolon>
 
           \<open>BinTree a\<^sub>E _ _\<close> \<open>BinTree a\<^sub>C\<^sub>R _ _\<close> \<m>\<a>\<k>\<e>\<s>(1) \<open>BinTree a\<^sub>D _ _\<close> \<semicolon>         (*for reasoning, \<Omega>*)
           \<open>BinTree a\<^sub>C\<^sub>L _ _\<close> \<open>BinTree a\<^sub>A _ _\<close> \<m>\<a>\<k>\<e>\<s>(1) \<open>BinTree a\<^sub>B _ _\<close> \<semicolon>         (*for reasoning, \<Omega>*)
@@ -530,62 +530,62 @@ proc maintain_i:
 
           holds_fact t1[useful]: \<open>k\<^sub>B < k\<^sub>D\<close>  \<semicolon>                                    (*for proof, Tac-s*)
 
-          return ($C) certified by (auto simp: map_add_def fun_eq_iff split: option.split; auto_sledgehammer)  (*Tac-1n-3m*)
+          return (C) certified by (auto simp: map_add_def fun_eq_iff split: option.split; auto_sledgehammer)  (*Tac-1n-3m*)
     \<medium_right_bracket>
   \<medium_right_bracket>
   \<medium_left_bracket>
-    if ($H\<^sub>E = $H\<^sub>B + 2) \<medium_left_bracket>
+    if (H\<^sub>E = H\<^sub>B + 2) \<medium_left_bracket>
 
       obtain F k\<^sub>E h\<^sub>E v\<^sub>E G where E[simp]: \<open>E = \<langle>F, (k\<^sub>E, h\<^sub>E, v\<^sub>E), G\<rangle>\<close> by auto_sledgehammer \<semicolon> (*for reasoning, \<Omega>*)
       \<open>BinTree a\<^sub>E _ _\<close> \<t>\<r>\<a>\<n>\<s>\<f>\<o>\<r>\<m>\<s>_\<t>\<o> \<open>\<o>\<p>\<e>\<n>(1)\<close> \<exists>a\<^sub>F, a\<^sub>G \<semicolon>
   
-      val F \<leftarrow> $E.left ! \<semicolon>
-      val G \<leftarrow> $E.right ! \<semicolon>
-      val H\<^sub>F \<leftarrow> height_of ($F) \<semicolon>
-      val H\<^sub>G \<leftarrow> height_of ($G) \<semicolon>
+      val F \<leftarrow> E.left \<semicolon>
+      val G \<leftarrow> E.right \<semicolon>
+      val H\<^sub>F \<leftarrow> height_of (F) \<semicolon>
+      val H\<^sub>G \<leftarrow> height_of (G) \<semicolon>
 
-      if ($H\<^sub>F \<le> $H\<^sub>G) \<medium_left_bracket>
+      if (H\<^sub>F \<le> H\<^sub>G) \<medium_left_bracket>
 
-          $a\<^sub>D.right := $F \<semicolon>
-          val H\<^sub>D' \<leftarrow> Max($H\<^sub>B, $H\<^sub>F) + 1 \<semicolon>
-          $a\<^sub>D.data.v.height := $H\<^sub>D' \<semicolon>
-          $E.left := $a\<^sub>D \<semicolon>
-          $E.data.v.height := Max($H\<^sub>D', $H\<^sub>G) + 1 \<semicolon>
+          a\<^sub>D.right := F \<semicolon>
+          val H\<^sub>D' \<leftarrow> Max(H\<^sub>B, H\<^sub>F) + 1 \<semicolon>
+          a\<^sub>D.data.v.height := H\<^sub>D' \<semicolon>
+          E.left := a\<^sub>D \<semicolon>
+          E.data.v.height := Max(H\<^sub>D', H\<^sub>G) + 1 \<semicolon>
 
           \<open>BinTree a\<^sub>F _ _\<close> \<open>BinTree a\<^sub>B _ _\<close> \<m>\<a>\<k>\<e>\<s>(1) \<open>BinTree a\<^sub>D _ _\<close> \<semicolon>                 (*for reasoning, \<Omega>*)
           \<m>\<a>\<k>\<e>\<s>(1) \<open>BinTree a\<^sub>E _ _\<close> \<semicolon>                                  (*for reasoning, \<Omega>*)
 
-          return ($E) certified by (auto simp: map_add_def fun_eq_iff split: option.split; auto_sledgehammer)  (*Tac-1n-3m*)
+          return (E) certified by (auto simp: map_add_def fun_eq_iff split: option.split; auto_sledgehammer)  (*Tac-1n-3m*)
       \<medium_right_bracket>
       \<medium_left_bracket>
           obtain F\<^sub>L k\<^sub>F h\<^sub>F v\<^sub>F F\<^sub>R where F[simp]: \<open>F = \<langle>F\<^sub>L, (k\<^sub>F, h\<^sub>F, v\<^sub>F), F\<^sub>R\<rangle>\<close> by auto_sledgehammer \<semicolon>
           \<open>BinTree a\<^sub>F _ _\<close> \<t>\<r>\<a>\<n>\<s>\<f>\<o>\<r>\<m>\<s>_\<t>\<o> \<open>\<o>\<p>\<e>\<n>(1)\<close> \<exists>a\<^sub>F\<^sub>L, a\<^sub>F\<^sub>R \<semicolon>
 
-          val F\<^sub>L \<leftarrow> $F.left ! \<semicolon>
-          val F\<^sub>R \<leftarrow> $F.right ! \<semicolon>
-          $a\<^sub>D.right := $F\<^sub>L \<semicolon>
-          val H\<^sub>D' \<leftarrow> Max ($H\<^sub>B, height_of ($F\<^sub>L)) + 1 \<semicolon>
-          $a\<^sub>D.data.v.height := $H\<^sub>D' \<semicolon>
-          $E.left := $F\<^sub>R \<semicolon>
-          val H\<^sub>E' \<leftarrow> Max (height_of ($F\<^sub>R), $H\<^sub>G) + 1 \<semicolon>
-          $E.data.v.height := $H\<^sub>E' \<semicolon>
-          $F.left := $a\<^sub>D \<semicolon>
-          $F.right := $E \<semicolon>
-          $F.data.v.height := Max($H\<^sub>D', $H\<^sub>E') + 1\<semicolon>
+          val F\<^sub>L \<leftarrow> F.left \<semicolon>
+          val F\<^sub>R \<leftarrow> F.right \<semicolon>
+          a\<^sub>D.right := F\<^sub>L \<semicolon>
+          val H\<^sub>D' \<leftarrow> Max (H\<^sub>B, height_of(F\<^sub>L)) + 1 \<semicolon>
+          a\<^sub>D.data.v.height := H\<^sub>D' \<semicolon>
+          E.left := F\<^sub>R \<semicolon>
+          val H\<^sub>E' \<leftarrow> Max (height_of(F\<^sub>R), H\<^sub>G) + 1 \<semicolon>
+          E.data.v.height := H\<^sub>E' \<semicolon>
+          F.left := a\<^sub>D \<semicolon>
+          F.right := E \<semicolon>
+          F.data.v.height := Max(H\<^sub>D', H\<^sub>E') + 1\<semicolon>
 
           \<open>BinTree a\<^sub>G _ _\<close> \<open>BinTree a\<^sub>F\<^sub>R _ _\<close> \<m>\<a>\<k>\<e>\<s>(1) \<open>BinTree a\<^sub>E _ _\<close> \<semicolon>
           \<open>BinTree a\<^sub>F\<^sub>L _ _\<close> \<open>BinTree a\<^sub>B _ _\<close> \<m>\<a>\<k>\<e>\<s>(1) \<open>BinTree a\<^sub>D _ _\<close> \<semicolon>
           \<m>\<a>\<k>\<e>\<s>(1) \<open>BinTree a\<^sub>F _ _\<close> \<semicolon>
 
-          return ($F) certified by (clarsimp, rule,
-                                    ((auto simp: map_add_def fun_eq_iff split: option.split)[1]; auto_sledgehammer),
-                                    auto; auto_sledgehammer)                          (*Tac-4n-3m*)
+          return (F) certified by (clarsimp, rule,
+                                   ((auto simp: map_add_def fun_eq_iff split: option.split)[1]; auto_sledgehammer),
+                                   auto; auto_sledgehammer)                          (*Tac-4n-3m*)
       \<medium_right_bracket>
     \<medium_right_bracket>
     \<medium_left_bracket>
-      $a\<^sub>D.data.v.height := Max (height_of ($a\<^sub>D.left !), height_of ($a\<^sub>D.right !)) + 1  \<semicolon>
+      a\<^sub>D.data.v.height := Max (height_of (a\<^sub>D.left), height_of (a\<^sub>D.right)) + 1  \<semicolon>
       \<open>BinTree a\<^sub>B _ _ \<close> \<m>\<a>\<k>\<e>\<s>(1) \<open>BinTree a\<^sub>D _ _\<close> \<semicolon>
-      return ($a\<^sub>D)
+      return (a\<^sub>D)
     \<medium_right_bracket>
   \<medium_right_bracket>
 \<medium_right_bracket> .
@@ -620,34 +620,34 @@ proc insert_avl_i:
 
   if \<open>$addr = 0\<close> \<medium_left_bracket>
       val ret \<leftarrow> calloc1 \<open>Avl_Node\<close> \<semicolon>
-      $ret.data.k := $k \<semicolon>
-      $ret.data.v.v := $v \<semicolon>
-      $ret.data.v.height := 1 \<semicolon>
+      ret.data.k := k \<semicolon>
+      ret.data.v.v := v \<semicolon>
+      ret.data.v.height := 1 \<semicolon>
       \<m>\<a>\<k>\<e>\<s>(1) \<open>\<langle>\<langle>\<rangle>, (k,1,v), \<langle>\<rangle>\<rangle> \<Ztypecolon> BinTree addrb (\<a>\<v>\<l>_\<p>\<a>\<i>\<r> TY\<^sub>K TY\<^sub>V) \<lbrace> k: K, v: \<lbrace> height: \<nat>, v: V \<rbrace> \<rbrace>\<close> \<semicolon>
-      return ($ret)
+      return (ret)
   \<medium_right_bracket>
   \<medium_left_bracket>
       obtain L k' h' v' R where tree_def[simp]: \<open>tree = \<langle>L, (k', h', v'), R\<rangle>\<close> by auto_sledgehammer \<semicolon>
       \<t>\<r>\<a>\<n>\<s>\<f>\<o>\<r>\<m>\<s>_\<t>\<o> \<open>\<o>\<p>\<e>\<n>(1)\<close> \<exists>a\<^sub>L, a\<^sub>R \<semicolon>
 
-      val k' \<leftarrow> $addr.data.k ! \<semicolon>
-      if (eq ($k', $k)) \<medium_left_bracket>
-        $addr.data.v.v := $v \<semicolon>
+      val k' \<leftarrow> addr.data.k \<semicolon>
+      if (eq (k', k)) \<medium_left_bracket>
+        addr.data.v.v := v \<semicolon>
         \<m>\<a>\<k>\<e>\<s>(1) \<open>BinTree addr _ _\<close>  \<semicolon>
-        return ($addr)
+        return (addr)
       \<medium_right_bracket> \<medium_left_bracket>
-        if (cmp ($k, $k')) \<medium_left_bracket>
-            insert_avl_i ($addr.left !, $k, $v) \<rightarrow> val a\<^sub>L' \<semicolon>
-            $addr.left := $a\<^sub>L' \<semicolon>
+        if (cmp (k, k')) \<medium_left_bracket>
+            insert_avl_i (addr.left, k, v) \<rightarrow> val a\<^sub>L' \<semicolon>
+            addr.left := a\<^sub>L' \<semicolon>
             \<m>\<a>\<k>\<e>\<s>(1) \<open>BinTree addr _ _\<close> \<semicolon>
-            return (maintain_i ($addr))
+            return (maintain_i (addr))
         \<medium_right_bracket>
         \<medium_left_bracket>
-            insert_avl_i ($addr.right !, $k, $v) \<rightarrow> val a\<^sub>R' \<semicolon>
-            $addr.right := $a\<^sub>R' \<semicolon>
+            insert_avl_i (addr.right, k, v) \<rightarrow> val a\<^sub>R' \<semicolon>
+            addr.right := a\<^sub>R' \<semicolon>
             \<open>BinTree a\<^sub>L _ _\<close> \<m>\<a>\<k>\<e>\<s>(1) \<open>BinTree addr _ _\<close> \<semicolon>
 
-            return (maintain_i ($addr))
+            return (maintain_i (addr))
         \<medium_right_bracket>
       \<medium_right_bracket>
   \<medium_right_bracket>
@@ -664,7 +664,7 @@ proc (nodef) insert_avl:
           \<s>\<u>\<b>\<j> addr'. \<top>\<close>
   unfolding AVL_Tree.unfold
 \<medium_left_bracket>
-  insert_avl_i ($addr, $k, $v)
+  insert_avl_i (addr, k, v)
 \<medium_right_bracket> .
 
 
